Std/Data/Option/Init/Lemmas.lean
@@ -1,0 +1,17 @@
+/-
+Copyright (c) 2022 Mario Carneiro. All rights reserved.
+Released under Apache 2.0 license as described in the file LICENSE.
+Authors: Mario Carneiro
+-/
+
+namespace Option
+
+/-!
+# Bootstrapping theorems for Option
+
+These are theorems used in the definitions of `Std.Data.List.Basic`.
+New theorems should be added to `Std.Data.Option.Lemmas` if they are not needed by the bootstrap.
+-/
+
+@[simp] theorem getD_none : getD none a = a := rfl
+@[simp] theorem getD_some : getD (some a) b = a := rfl
